HoSmt/Decode/Rules.lean
@@ -1,0 +1,14 @@
+import Duper.Tactic
+
+namespace HoSmt.Decode.Rules
+
+/-- The Alethe2 proof rule `equiv_pos2`. -/
+theorem equiv_pos2 (α β : Prop) : α ≠ β ∨ ¬α ∨ β := by
+  match Classical.em α with
+  | Or.inl hα =>
+    match Classical.em β with
+    | Or.inl hβ => exact Or.inr (Or.inr hβ)
+    | Or.inr hβ => simp only [hα, hβ, ne_eq, not_true, true_or]
+  | Or.inr hα => exact Or.inr (Or.inl hα)
+
+end HoSmt.Decode.Rules
