HoSmt/Tests/PropLogic.lean
@@ -1,51 +1,101 @@
 import HoSmt
--- import Std.Logic
+import Duper.Tactic
+import HoSmt.Decode.Rules
+
+open HoSmt.Decode.Rules
 
 set_option trace.HoSmt true
+set_option trace.HoSmt.Decode true
+set_option HoSmt.reconstruct true
 
-abbrev Cl : List Prop -> Prop
-| [] => False
-| [x] => x
-| x :: xs => x ∨ (Cl xs)
+set_option linter.unusedVariables false
 
-def add (a b : Nat) : Nat := a + b
+theorem test : True ∨ False := by smt
+#print axioms test
+example : True ∨ False ∨ False  := by smt
+example : False ∨ (True = ¬False) := by smt
 
-#check Nat
+open HoSmt.Decode.Alethe2
+theorem test2 : ∀x: Prop, x = x := by smtProof
+  unsat
+  (assume a0 (not (forall ((VAR_x Bool)) (= VAR_x VAR_x))))
+  (assume a1 true)
+  (step t1 (cl (not (= (not (forall ((VAR_x Bool)) (= VAR_x VAR_x))) false)) (not (not (forall ((VAR_x Bool)) (= VAR_x VAR_x)))) false) :rule equiv_pos2)
+  
+  (anchor :step t2 :args ((:= (VAR_x Bool) VAR_x)))
+  (step t2.t1 (cl (= VAR_x VAR_x)) :rule refl)
+  (step t2.t2 (cl (= (= VAR_x VAR_x) true)) :rule all_simplify)
+  (step t2 (cl (= (forall ((VAR_x Bool)) (= VAR_x VAR_x)) (forall ((VAR_x Bool)) true))) :rule bind)
+  
+  (step t3 (cl (= (forall ((VAR_x Bool)) true) true)) :rule all_simplify)
+  (step t4 (cl (= (forall ((VAR_x Bool)) (= VAR_x VAR_x)) true)) :rule trans :premises (t2 t3))
+  (step t5 (cl (= (not (forall ((VAR_x Bool)) (= VAR_x VAR_x))) (not true))) :rule cong :premises (t4))
+  (step t6 (cl (= (not true) false)) :rule all_simplify)
+  (step t7 (cl (= (not (forall ((VAR_x Bool)) (= VAR_x VAR_x))) false)) :rule trans :premises (t5 t6))
+  (step t8 (cl) :rule resolution :premises (t1 t7 a0))
 
-theorem cl_yes {xs : List Prop} (h : x) : x ∈ xs -> Cl xs := by sorry
+example : ∀x: Prop, x = x := by smt
 
-theorem equiv_pos2 (α β : Prop) : Cl [α ≠ β, ¬α, β] := by sorry
-  -- match Classical.em α with
-  -- | Or.inl h =>
-  --   match Classical.em (α = β) with
-  --   | Or.inl h₂ => sorry 
-  --   | Or.inr h₂ => simp; exact cl_yes h₂ (List.Mem.head _)
-  -- | Or.inr h => exact cl_yes h (List.Mem.tail _ (List.Mem.head _))
+example : ∀x, False ∨ (x = True) ∨ (x = ¬True) := by smtProof
+  unsat
+  (assume a0 (not (forall ((VAR_x Bool)) (or false (or (= VAR_x true) (= VAR_x (not true)))))))
+  (assume a1 true)
+  (step t1 (cl
+    (not (= (not (forall ((VAR_x Bool)) (or false (or (= VAR_x true) (= VAR_x (not true)))))) false))
+    (not (not (forall ((VAR_x Bool)) (or false (or (= VAR_x true) (= VAR_x (not true))))))) false)
+    :rule equiv_pos2)
+  (anchor :step t2 :args ((:= (VAR_x Bool) VAR_x)))
+  (step t2.t1 (cl (= VAR_x VAR_x)) :rule refl)
+  (step t2.t2 (cl (= (or false (or (= VAR_x true) (= VAR_x (not true)))) (or (= VAR_x true) (= VAR_x (not true))))) :rule all_simplify)
+  (step t2.t3 (cl (= (= VAR_x true) VAR_x)) :rule all_simplify)
+  (step t2.t4 (cl (= VAR_x VAR_x)) :rule refl)
+  (step t2.t5 (cl (= (not true) false)) :rule all_simplify)
+  (step t2.t6 (cl (= (= VAR_x (not true)) (= VAR_x false))) :rule cong :premises (t2.t4 t2.t5))
+  (step t2.t7 (cl (= (= VAR_x false) (not VAR_x))) :rule all_simplify)
+  (step t2.t8 (cl (= (= VAR_x (not true)) (not VAR_x))) :rule trans :premises (t2.t6 t2.t7))
+  (step t2.t9 (cl (= (or (= VAR_x true) (= VAR_x (not true))) (or VAR_x (not VAR_x)))) :rule cong :premises (t2.t3 t2.t8))
+  (step t2.t10 (cl (= (or false (or (= VAR_x true) (= VAR_x (not true)))) (or VAR_x (not VAR_x)))) :rule trans :premises (t2.t2 t2.t9))
+  (step t2 (cl (= (forall ((VAR_x Bool)) (or false (or (= VAR_x true) (= VAR_x (not true))))) (forall ((VAR_x Bool)) (or VAR_x (not VAR_x))))) :rule bind)
+  (step t3 (cl (= (forall ((VAR_x Bool)) (or VAR_x (not VAR_x))) (forall ((VAR_x Bool)) true))) :rule all_simplify)
+  (step t4 (cl (= (forall ((VAR_x Bool)) true) true)) :rule all_simplify)
+  (step t5 (cl (= (forall ((VAR_x Bool)) (or VAR_x (not VAR_x))) true)) :rule trans :premises (t3 t4))
+  (step t6 (cl (= (forall ((VAR_x Bool)) (or false (or (= VAR_x true) (= VAR_x (not true))))) true)) :rule trans :premises (t2 t5))
+  (step t7 (cl (= (not (forall ((VAR_x Bool)) (or false (or (= VAR_x true) (= VAR_x (not true)))))) (not true))) :rule cong :premises (t6))
+  (step t8 (cl (= (not true) false)) :rule all_simplify)
+  (step t9 (cl (= (not (forall ((VAR_x Bool)) (or false (or (= VAR_x true) (= VAR_x (not true)))))) false)) :rule trans :premises (t7 t8))
+  (step t10 (cl) :rule resolution :premises (t1 t9 a0))
 
-/-
-unsat
-(assume a0 (not (or true false)))
-(assume a1 true)
-(step t1 (cl (not (= (not (or true false)) false)) (not (not (or true false))) false) :rule equiv_pos2)
-(step t2 (cl (= (or true false) true)) :rule all_simplify)
-(step t3 (cl (= (not (or true false)) (not true))) :rule cong :premises (t2))
-(step t4 (cl (= (not true) false)) :rule all_simplify)
-(step t5 (cl (= (not (or true false)) false)) :rule trans :premises (t3 t4))
-(step t6 (cl) :rule resolution :premises (t1 t5 a0))
+/- Generates the following TPTP input:
+% inductive Nat : Type
+thf(ty0, type, glob_Nat : $tType).
+% ctor Nat.zero : Nat
+thf(ty1, type, glob_Nat_zero : glob_Nat).
+% ctor Nat.succ : Nat -> Nat
+thf(ty2, type, glob_Nat_succ : (glob_Nat > glob_Nat)).
+% axiom Nat.succ.injEq : forall (n : Nat) (n_1 : Nat), Eq.{1} Prop (Eq.{1} Nat (Nat.succ n) (Nat.succ n_1)) (Eq.{1} Nat n n_1)
+thf(ax3, axiom, (![VAR_n : glob_Nat]: (![VAR_n__uniq_39302 : glob_Nat]: (((glob_Nat_succ @ VAR_n) = (glob_Nat_succ @ VAR_n__uniq_39302)) = (VAR_n = VAR_n__uniq_39302))))).
+thf(goal, conjecture, (![VAR_n : glob_Nat]: (VAR_n = VAR_n))).
 -/
-example : Or True False := by smt
+set_option HoSmt.reconstruct false in
+example : ∀n : Nat, n = n := by smt
 
-example : True ∨ False := by
-  have f (a0 : ¬(True ∨ False)) : False := by
-    have t1 : Cl [(¬(True ∨ False)) ≠ False, ¬¬(True ∨ False), False] := by exact equiv_pos2 (¬(True ∨ False)) False
-    have t2 : Cl [(True ∨ False) = True] := by simp
-    have t3 : Cl [(¬(True ∨ False)) = ¬True] := by simp [t2]
-    have t4 : Cl [(¬True) = False] := by simp
-    have t5 : Cl [(¬ True ∨ False) = False] := by simp
-    have t6 : Cl [] := by simp at a0
-    exact t6
-  simp
-#check Classical.not_not
-
-#cvc5 "thf(goal, conjecture, $true | $false)."
+-- example : ∀n : Nat, n = n := by
+--   smtProof
+--     unsat
+--     -- TODO: Problem is this extra assume, which doesn't vibe with smt_harness
+--     (assume a0 (forall ((VAR_n glob_Nat)) (forall ((VAR_n__uniq_39302 glob_Nat)) (= (= (@ glob_Nat_succ VAR_n) (@ glob_Nat_succ VAR_n__uniq_39302)) (= VAR_n VAR_n__uniq_39302)))))
+--     (assume a1 (not (forall ((VAR_n glob_Nat)) (= VAR_n VAR_n))))
+--     (assume a2 true)
+--     (step t1 (cl (not (= (not (forall ((VAR_n glob_Nat)) (= VAR_n VAR_n))) false)) (not (not (forall ((VAR_n glob_Nat)) (= VAR_n VAR_n)))) false) :rule equiv_pos2)
+--     (anchor :step t2 :args ((:= (VAR_n glob_Nat) VAR_n)))
+--     (step t2.t1 (cl (= VAR_n VAR_n)) :rule refl)
+--     (step t2.t2 (cl (= (= VAR_n VAR_n) true)) :rule all_simplify)
+--     (step t2 (cl (= (forall ((VAR_n glob_Nat)) (= VAR_n VAR_n)) (forall ((VAR_n glob_Nat)) true))) :rule bind)
+--     (step t3 (cl (= (forall ((VAR_n glob_Nat)) true) true)) :rule all_simplify)
+--     (step t4 (cl (= (forall ((VAR_n glob_Nat)) (= VAR_n VAR_n)) true)) :rule trans :premises (t2 t3))
+--     (step t5 (cl (= (not (forall ((VAR_n glob_Nat)) (= VAR_n VAR_n))) (not true))) :rule cong :premises (t4))
+--     (step t6 (cl (= (not true) false)) :rule all_simplify)
+--     (step t7 (cl (= (not (forall ((VAR_n glob_Nat)) (= VAR_n VAR_n))) false)) :rule trans :premises (t5 t6))
+--     (step t8 (cl) :rule resolution :premises (t1 t7 a1))
+--   done
 
