HoSmt/Tests/Tests.lean
@@ -1,3 +1,0 @@
-import HoSmt.Tests.Vec
-import HoSmt.Tests.HigherOrder
-import HoSmt.Tests.PredToInductive
