HoSmt/Tests/Vec.lean
@@ -5,10 +5,11 @@ set_option trace.HoSmt true
 
 theorem simple : ∀v : Vec Nat n, v = v := by smt
 
-
 inductive All (P : α -> Prop) : Vec α n -> Prop
 | nil : All P Vec.nil
 | cons : P x -> All P xs -> All P (Vec.cons x xs)
 
+-- The following translates but cvc5 fails to find a proof :(
+set_option HoSmt.shouldTranslate true in
 example: ∀v : Vec Nat n, All (. <= 10) v -> sum v <= 10 * n := by smt
 
