lakefile.lean
@@ -3,7 +3,12 @@ open Lake DSL
 
 package HoSmt
 
--- Only needed for tests:
-require mathlib from git "https://github.com/leanprover-community/mathlib4"
+require std from git "https://github.com/leanprover/std4"@"main"
 
+require Duper from git "https://github.com/leanprover-community/duper"@"main"
+
+-- Only needed for tests:
+require mathlib from git "https://github.com/leanprover-community/mathlib4"@"master"
+
+@[default_target]
 lean_lib HoSmt
